Soundness.v
@@ -6,6 +6,26 @@ Require Import Typing.
 Require Import Constraint.
 Require Import TypeSubst.
 
+Lemma lambda_solution: forall tsubst T S T1 T2 tenv x t C,
+  Constraint.Solution tsubst T tenv (Lambda x T1 t) (FunT T1 T2) C ->
+  TypeSubst T2 S tsubst ->
+  Constraint.Solution tsubst S (TEnv.add x T1 tenv) t T2 C.
+Proof.
+unfold Constraint.Solution in |- *.
+intros.
+inversion H.
+split.
+ inversion H1.
+ exact H10.
+
+ inversion H2.
+ split.
+  exact H3.
+
+  exact H0.
+Qed.
+
+
 Theorem soundness : forall tenv t T S C tsubst,
   TypeConstraint t tenv S nil C ->
   Constraint.Solution tsubst T tenv t S C ->
@@ -15,3 +35,35 @@ intros until tsubst.
 intro.
 pattern t, tenv, S, (nil:tvars), C in |- *.
 apply TypeConstraint_ind.
+ intros.
+ unfold Solution in |- *.
+ intros.
+ apply
+  subst_preserve
+   with (tsubst := tsubst) (t := Var s) (tenv1 := tenv0) (T := T0).
+  apply TVar.
+  exact H0.
+
+  exact H2.
+
+  exact H3.
+
+  unfold Constraint.Solution in H1.
+  inversion H1.
+  inversion H5.
+  exact H7.
+
+(*intros.
+unfold Solution in |- *.
+intros.
+apply
+ subst_preserve
+  with (tsubst := tsubst) (t := Var s) (tenv1 := tenv0) (T := T0).
+ apply TVar.
+ exact H0.
+
+ exact H2.
+
+ exact H3.
+
+*)
